Minor changes (WIP)

coq/src/Concordium_template.v
@@ -9,21 +9,543 @@ Open Scope hacspec_scope.
 (* Coq code:1 ends here *)
 
 (* [[file:concordium.org::*Coq code][Coq code:2]] *)
-Definition max_contract_state_size_v : int32 :=
-  @repr WORDSIZE32 16384.
+Require Import Hacspec.Lib.
 (* Coq code:2 ends here *)
 
 (* [[file:concordium.org::*Coq code][Coq code:3]] *)
-Definition max_log_size_v : uint_size :=
-  usize 512.
+Definition max_contract_state_size_v : int32 :=
+  @repr WORDSIZE32 16384.
 (* Coq code:3 ends here *)
 
 (* [[file:concordium.org::*Coq code][Coq code:4]] *)
-Definition max_num_logs_v : uint_size :=
-  usize 64.
+Definition max_log_size_v : uint_size :=
+  usize 512.
 (* Coq code:4 ends here *)
 
 (* [[file:concordium.org::*Coq code][Coq code:5]] *)
+Definition max_num_logs_v : uint_size :=
+  usize 64.
+(* Coq code:5 ends here *)
+
+(* [[file:concordium.org::*Coq code][Coq code:6]] *)
+Notation "'reject_hacspec_t'" := (int32) : hacspec_scope.
+(* Coq code:6 ends here *)
+
+(* [[file:concordium.org::*Coq code][Coq code:7]] *)
+Definition reject_impl_deafult  : reject_hacspec_t :=
+  min_v.
+(* Coq code:7 ends here *)
+
+(* [[file:concordium.org::*Coq code][Coq code:8]] *)
+Definition new_reject_impl (x_0 : int32) : (option int32) :=
+  (if ((x_0) <.? (@repr WORDSIZE32 0)):bool then (@Some int32 (x_0)) else (
+      @None int32)).
+(* Coq code:8 ends here *)
+
+(* [[file:concordium.org::*Coq code][Coq code:9]] *)
+Definition reject_impl_convert_from_unit  : reject_hacspec_t :=
+  (min_v) .+ (@repr WORDSIZE32 1).
+
+Theorem ensures_reject_impl_convert_from_unit : forall result_1 ,
+@reject_impl_convert_from_unit  = result_1 ->
+~ (result_1 = @repr WORDSIZE32 0).
+Proof. Admitted.
+(* Coq code:9 ends here *)
+
+(* [[file:concordium.org::*Coq code][Coq code:10]] *)
+Definition reject_impl_convert_from_parse_error  : reject_hacspec_t :=
+  (min_v) .+ (@repr WORDSIZE32 2).
+
+Theorem ensures_reject_impl_convert_from_parse_error : forall result_1 ,
+@reject_impl_convert_from_parse_error  = result_1 ->
+~ (result_1 = @repr WORDSIZE32 0).
+Proof. Admitted.
+(* Coq code:10 ends here *)
+
+(* [[file:concordium.org::*Coq code][Coq code:11]] *)
+Definition reject_impl_from_log_error (le_2 : log_error_t) : reject_hacspec_t :=
+  match le_2 with
+  | Full => (min_v) .+ (@repr WORDSIZE32 3)
+  | Malformed => (min_v) .+ (@repr WORDSIZE32 4)
+  end.
+
+Theorem ensures_reject_impl_from_log_error : forall result_1 (
+  le_2 : log_error_t),
+@reject_impl_from_log_error le_2 = result_1 ->
+~ (result_1 = @repr WORDSIZE32 0).
+Proof. Admitted.
+(* Coq code:11 ends here *)
+
+(* [[file:concordium.org::*Coq code][Coq code:12]] *)
+Inductive new_contract_name_error_t :=
+| NewContractNameErrorMissingInitPrefix : new_contract_name_error_t
+| NewContractNameErrorTooLong : new_contract_name_error_t
+| NewContractNameErrorContainsDot : new_contract_name_error_t
+| NewContractNameErrorInvalidCharacters : new_contract_name_error_t.
+(* Coq code:12 ends here *)
+
+(* [[file:concordium.org::*Coq code][Coq code:13]] *)
+Definition reject_impl_from_new_contract_name_error
+  (nre_3 : new_contract_name_error_t)
+  : reject_hacspec_t :=
+  match nre_3 with
+  | NewContractNameErrorMissingInitPrefix => (min_v) .+ (@repr WORDSIZE32 5)
+  | NewContractNameErrorTooLong => (min_v) .+ (@repr WORDSIZE32 6)
+  | NewContractNameErrorContainsDot => (min_v) .+ (@repr WORDSIZE32 9)
+  | NewContractNameErrorInvalidCharacters => (min_v) .+ (@repr WORDSIZE32 10)
+  end.
+
+Theorem ensures_reject_impl_from_new_contract_name_error : forall result_1 (
+  nre_3 : new_contract_name_error_t),
+@reject_impl_from_new_contract_name_error nre_3 = result_1 ->
+~ (result_1 = @repr WORDSIZE32 0).
+Proof. Admitted.
+(* Coq code:13 ends here *)
+
+(* [[file:concordium.org::*Coq code][Coq code:14]] *)
+Inductive new_receive_name_error_t :=
+| NewReceiveNameErrorMissingDotSeparator : new_receive_name_error_t
+| NewReceiveNameErrorTooLong : new_receive_name_error_t
+| NewReceiveNameErrorInvalidCharacters : new_receive_name_error_t.
+(* Coq code:14 ends here *)
+
+(* [[file:concordium.org::*Coq code][Coq code:15]] *)
+Definition reject_impl_from_new_receive_name_error
+  (nre_4 : new_receive_name_error_t)
+  : reject_hacspec_t :=
+  match nre_4 with
+  | NewReceiveNameErrorMissingDotSeparator => (min_v) .+ (@repr WORDSIZE32 7)
+  | NewReceiveNameErrorTooLong => (min_v) .+ (@repr WORDSIZE32 8)
+  | NewReceiveNameErrorInvalidCharacters => (min_v) .+ (@repr WORDSIZE32 11)
+  end.
+
+Theorem ensures_reject_impl_from_new_receive_name_error : forall result_1 (
+  nre_4 : new_receive_name_error_t),
+@reject_impl_from_new_receive_name_error nre_4 = result_1 ->
+~ (result_1 = @repr WORDSIZE32 0).
+Proof. Admitted.
+(* Coq code:15 ends here *)
+
+(* [[file:concordium.org::*Coq code][Coq code:16]] *)
+Notation "'contract_state_hacspec_t'" := (int32) : hacspec_scope.
+(* Coq code:16 ends here *)
+
+(* [[file:concordium.org::*Coq code][Coq code:17]] *)
+Inductive seek_from_hacspec_t :=
+| Start : int64 -> seek_from_hacspec_t
+| End : int64 -> seek_from_hacspec_t
+| Current : int64 -> seek_from_hacspec_t.
+(* Coq code:17 ends here *)
+
+(* [[file:concordium.org::*Coq code][Coq code:18]] *)
+Notation "'uint32_option_t'" := ((option int32)) : hacspec_scope.
+(* Coq code:18 ends here *)
+
+(* [[file:concordium.org::*Coq code][Coq code:19]] *)
+Notation "'iint64_option_t'" := ((option int64)) : hacspec_scope.
+(* Coq code:19 ends here *)
+
+(* [[file:concordium.org::*Coq code][Coq code:20]] *)
+Definition contract_state_impl_seek
+  (current_position_5 : contract_state_hacspec_t)
+  (pos_6 : seek_from_hacspec_t)
+  : (result (contract_state_hacspec_t × int64) unit) :=
+  match pos_6 with
+  | Start offset_7 => @Ok (contract_state_hacspec_t × int64) unit ((
+      @cast _ uint32 _ (offset_7),
+      offset_7
+    ))
+  | End delta_8 => (if ((delta_8) >=.? (@repr WORDSIZE64 0)):bool then (
+      match pub_uint32_checked_add (current_position_5) (@cast _ uint32 _ (
+          delta_8)) with
+      | Some b_9 => @Ok (contract_state_hacspec_t × int64) unit ((
+          b_9,
+          @cast _ uint64 _ (delta_8)
+        ))
+      | None => @Err (contract_state_hacspec_t × int64) unit (tt)
+      end) else (match pub_int64_checked_abs (delta_8) with
+      | Some b_10 => @Ok (contract_state_hacspec_t × int64) unit ((
+          (@repr WORDSIZE32 4) .- (@cast _ uint32 _ (b_10)),
+          @cast _ uint64 _ ((@repr WORDSIZE32 4) .- (@cast _ uint32 _ (b_10)))
+        ))
+      | None => @Err (contract_state_hacspec_t × int64) unit (tt)
+      end))
+  | Current delta_11 => (if ((delta_11) >=.? (@repr WORDSIZE64 0)):bool then (
+      match pub_uint32_checked_add (current_position_5) (@cast _ uint32 _ (
+          delta_11)) with
+      | Some offset_12 => @Ok (contract_state_hacspec_t × int64) unit ((
+          offset_12,
+          @cast _ uint64 _ (offset_12)
+        ))
+      | None => @Err (contract_state_hacspec_t × int64) unit (tt)
+      end) else (match pub_int64_checked_abs (delta_11) with
+      | Some b_13 => match pub_uint32_checked_sub (current_position_5) (
+        @cast _ uint32 _ (b_13)) with
+      | Some offset_14 => @Ok (contract_state_hacspec_t × int64) unit ((
+          offset_14,
+          @cast _ uint64 _ (offset_14)
+        ))
+      | None => @Err (contract_state_hacspec_t × int64) unit (tt)
+      end
+      | None => @Err (contract_state_hacspec_t × int64) unit (tt)
+      end))
+  end.
+(* Coq code:20 ends here *)
+
+(* [[file:concordium.org::*Coq code][Coq code:21]] *)
+Definition contract_state_impl_read_read
+  (current_position_15 : contract_state_hacspec_t)
+  (buf_16 : public_byte_seq)
+  : (contract_state_hacspec_t × uint_size) :=
+  let '(buf_17, num_read_18) :=
+    load_state_hacspec (buf_16) (current_position_15) in 
+  ((current_position_15) .+ (num_read_18), @cast _ uint32 _ (num_read_18)).
+(* Coq code:21 ends here *)
+
+(* [[file:concordium.org::*Coq code][Coq code:22]] *)
+Definition contract_state_impl_read_read_u64
+  (current_position_19 : contract_state_hacspec_t)
+  : (contract_state_hacspec_t × int64) :=
+  let buf_20 : seq int8 :=
+    seq_new_ (default) (usize 8) in 
+  let '(buf_21, num_read_22) :=
+    load_state_hacspec (buf_20) (current_position_19) in 
+  (
+    (current_position_19) .+ (num_read_22),
+    u64_from_le_bytes (array_from_seq (8) (buf_21))
+  ).
+(* Coq code:22 ends here *)
+
+(* [[file:concordium.org::*Coq code][Coq code:23]] *)
+Definition contract_state_impl_read_read_u32
+  (current_position_23 : contract_state_hacspec_t)
+  : (contract_state_hacspec_t × int32) :=
+  let buf_24 : seq int8 :=
+    seq_new_ (default) (usize 4) in 
+  let '(buf_25, num_read_26) :=
+    load_state_hacspec (buf_24) (current_position_23) in 
+  (
+    (current_position_23) .+ (num_read_26),
+    u32_from_le_bytes (array_from_seq (4) (buf_25))
+  ).
+(* Coq code:23 ends here *)
+
+(* [[file:concordium.org::*Coq code][Coq code:24]] *)
+Definition contract_state_impl_read_read_u8
+  (current_position_27 : contract_state_hacspec_t)
+  : (contract_state_hacspec_t × int8) :=
+  let buf_28 : seq int8 :=
+    seq_new_ (default) (usize 1) in 
+  let '(buf_29, num_read_30) :=
+    load_state_hacspec (buf_28) (current_position_27) in 
+  ((current_position_27) .+ (num_read_30), seq_index (buf_29) (usize 0)).
+(* Coq code:24 ends here *)
+
+(* [[file:concordium.org::*Coq code][Coq code:25]] *)
+Definition contract_state_impl_write
+  (current_position_31 : contract_state_hacspec_t)
+  (buf_32 : public_byte_seq)
+  : (result (contract_state_hacspec_t × uint_size) unit) :=
+  ifbnd option_is_none (pub_uint32_checked_add (current_position_31) (pub_u32 (
+        seq_len (buf_32)))) : bool
+  thenbnd (bind (@Err (contract_state_hacspec_t × uint_size) unit (tt)) (
+      fun _ =>  Ok (tt)))
+  else (tt) >> (fun 'tt =>
+  let '(buf_33, num_bytes_34) :=
+    write_state_hacspec (buf_32) (current_position_31) in 
+  @Ok (contract_state_hacspec_t × uint_size) unit ((
+      (current_position_31) .+ (num_bytes_34),
+      @cast _ uint32 _ (num_bytes_34)
+    ))).
+(* Coq code:25 ends here *)
+
+(* [[file:concordium.org::*Coq code][Coq code:26]] *)
+Definition has_contract_state_impl_for_contract_state_open
+  
+  : contract_state_hacspec_t :=
+  @repr WORDSIZE32 0.
+(* Coq code:26 ends here *)
+
+(* [[file:concordium.org::*Coq code][Coq code:27]] *)
+Definition has_contract_state_impl_for_contract_state_reserve
+  (len_35 : int32)
+  : bool :=
+  let cur_size_36 : int32 :=
+    state_size_hacspec  in 
+  (if ((cur_size_36) <.? (len_35)):bool then ((resize_state_hacspec (
+          len_35)) =.? (@repr WORDSIZE32 1)) else (true)).
+(* Coq code:27 ends here *)
+
+(* [[file:concordium.org::*Coq code][Coq code:28]] *)
+Definition has_contract_state_impl_for_contract_state_truncate
+  (current_position_37 : contract_state_hacspec_t)
+  (cur_size_38 : int32)
+  (new_size_39 : int32)
+  : contract_state_hacspec_t :=
+  let 'tt :=
+    if (cur_size_38) >.? (new_size_39):bool then (let _ : int32 :=
+        resize_state_hacspec (new_size_39) in 
+      tt) else (tt) in 
+  (if ((new_size_39) <.? (current_position_37)):bool then (new_size_39) else (
+      current_position_37)).
+(* Coq code:28 ends here *)
+
+(* [[file:concordium.org::*Coq code][Coq code:29]] *)
+Notation "'parameter_hacspec_t'" := (int32) : hacspec_scope.
+(* Coq code:29 ends here *)
+
+(* [[file:concordium.org::*Coq code][Coq code:30]] *)
+Definition read_impl_for_parameter_read
+  (current_position_40 : parameter_hacspec_t)
+  (buf_41 : public_byte_seq)
+  : (parameter_hacspec_t × uint_size) :=
+  let '(buf_42, num_read_43) :=
+    get_parameter_section_hacspec (buf_41) (current_position_40) in 
+  ((current_position_40) .+ (num_read_43), @cast _ uint32 _ (num_read_43)).
+(* Coq code:30 ends here *)
+
+(* [[file:concordium.org::*Coq code][Coq code:31]] *)
+Notation "'attributes_cursor_hacspec_t'" := ((int32 × int16)) : hacspec_scope.
+(* Coq code:31 ends here *)
+
+(* [[file:concordium.org::*Coq code][Coq code:32]] *)
+Definition has_policy_impl_for_policy_attributes_cursor_next_item
+  (policy_attribute_items_44 : attributes_cursor_hacspec_t)
+  (buf_45 : public_byte_seq)
+  : (option (attributes_cursor_hacspec_t × (int8 × int8))) :=
+  let '(current_position_46, remaining_items_47) :=
+    policy_attribute_items_44 in 
+  ifbnd (remaining_items_47) =.? (@repr WORDSIZE16 0) : bool
+  thenbnd (bind (@None (attributes_cursor_hacspec_t × (int8 × int8))) (
+      fun _ =>  Some (tt)))
+  else (tt) >> (fun 'tt =>
+  let '(tag_value_len_48, num_read_49) :=
+    get_policy_section_hacspec (seq_new_ (default) (usize 2)) (
+      current_position_46) in 
+  let current_position_46 :=
+    (current_position_46) .+ (num_read_49) in 
+  ifbnd (seq_index (tag_value_len_48) (usize 1)) >.? (@repr WORDSIZE8 31) : bool
+  thenbnd (bind (@None (attributes_cursor_hacspec_t × (int8 × int8))) (
+      fun _ =>  Some (tt)))
+  else (tt) >> (fun 'tt =>
+  let '(buf_50, num_read_51) :=
+    get_policy_section_hacspec (buf_45) (current_position_46) in 
+  let current_position_46 :=
+    (current_position_46) .+ (num_read_51) in 
+  let remaining_items_47 :=
+    (remaining_items_47) .- (@repr WORDSIZE16 1) in 
+  @Some (attributes_cursor_hacspec_t × (int8 × int8)) ((
+      (current_position_46, remaining_items_47),
+      (
+        seq_index (tag_value_len_48) (usize 0),
+        seq_index (tag_value_len_48) (usize 1)
+      )
+    )))).
+(* Coq code:32 ends here *)
+
+(* [[file:concordium.org::*Coq code][Coq code:33]] *)
+Notation "'policies_iterator_hacspec_t'" := ((int32 × int16)) : hacspec_scope.
+(* Coq code:33 ends here *)
+
+(* [[file:concordium.org::*Coq code][Coq code:34]] *)
+Notation "'policy_attributes_cursor_hacspec_t'" := ((
+  int32 ×
+  int64 ×
+  int64 ×
+  attributes_cursor_hacspec_t
+)) : hacspec_scope.
+(* Coq code:34 ends here *)
+
+(* [[file:concordium.org::*Coq code][Coq code:35]] *)
+Definition iterator_impl_for_policies_iterator_next
+  (policies_iterator_52 : policies_iterator_hacspec_t)
+  : (option (policies_iterator_hacspec_t × policy_attributes_cursor_hacspec_t
+    )) :=
+  let '(pos_53, remaining_items_54) :=
+    policies_iterator_52 in 
+  ifbnd (remaining_items_54) =.? (@repr WORDSIZE16 0) : bool
+  thenbnd (bind (@None (
+        policies_iterator_hacspec_t ×
+        policy_attributes_cursor_hacspec_t
+      )) (fun _ =>  Some (tt)))
+  else (tt) >> (fun 'tt =>
+  let '(buf_55, _) :=
+    get_policy_section_hacspec (seq_new_ (default) (((((usize 2) + (
+                usize 4)) + (usize 8)) + (usize 8)) + (usize 2))) (pos_53) in 
+  let skip_part_56 : public_byte_seq :=
+    seq_slice_range (buf_55) ((usize 0, usize 2)) in 
+  let ip_part_57 : public_byte_seq :=
+    seq_slice_range (buf_55) ((usize 2, (usize 2) + (usize 4))) in 
+  let created_at_part_58 : public_byte_seq :=
+    seq_slice_range (buf_55) ((
+        (usize 2) + (usize 4),
+        ((usize 2) + (usize 4)) + (usize 8)
+      )) in 
+  let valid_to_part_59 : public_byte_seq :=
+    seq_slice_range (buf_55) ((
+        ((usize 2) + (usize 4)) + (usize 8),
+        (((usize 2) + (usize 4)) + (usize 8)) + (usize 8)
+      )) in 
+  let len_part_60 : public_byte_seq :=
+    seq_slice_range (buf_55) ((
+        (((usize 2) + (usize 4)) + (usize 8)) + (usize 8),
+        ((((usize 2) + (usize 4)) + (usize 8)) + (usize 8)) + (usize 2)
+      )) in 
+  let identity_provider_61 : int32 :=
+    u32_from_le_bytes (array_from_seq (4) (ip_part_57)) in 
+  let created_at_62 : int64 :=
+    u64_from_le_bytes (array_from_seq (8) (created_at_part_58)) in 
+  let valid_to_63 : int64 :=
+    u64_from_le_bytes (array_from_seq (8) (valid_to_part_59)) in 
+  let remaining_items_64 : int16 :=
+    u16_from_le_bytes (array_from_seq (2) (len_part_60)) in 
+  let attributes_start_65 : int32 :=
+    (((((pos_53) .+ (@repr WORDSIZE32 2)) .+ (@repr WORDSIZE32 4)) .+ (
+          @repr WORDSIZE32 8)) .+ (@repr WORDSIZE32 8)) .+ (
+      @repr WORDSIZE32 2) in 
+  let pos_53 :=
+    ((pos_53) .+ (@cast _ uint32 _ (u16_from_le_bytes (array_from_seq (2) (
+              skip_part_56))))) .+ (@repr WORDSIZE32 2) in 
+  let remaining_items_64 :=
+    (remaining_items_64) .- (@repr WORDSIZE16 1) in 
+  @Some (policies_iterator_hacspec_t × policy_attributes_cursor_hacspec_t) ((
+      (pos_53, remaining_items_64),
+      (
+        identity_provider_61,
+        created_at_62,
+        valid_to_63,
+        (attributes_start_65, remaining_items_64)
+      )
+    ))).
+(* Coq code:35 ends here *)
+
+(* [[file:concordium.org::*Coq code][Coq code:36]] *)
+Definition load_state_hacspec
+  (buf_66 : public_byte_seq)
+  (offset_67 : int32)
+  : (public_byte_seq × int32) :=
+  (buf_66, @repr WORDSIZE32 1).
+(* Coq code:36 ends here *)
+
+(* [[file:concordium.org::*Coq code][Coq code:37]] *)
+Definition write_state_hacspec
+  (buf_68 : public_byte_seq)
+  (offset_69 : int32)
+  : (public_byte_seq × int32) :=
+  (buf_68, @repr WORDSIZE32 1).
+(* Coq code:37 ends here *)
+
+(* [[file:concordium.org::*Coq code][Coq code:38]] *)
+Definition state_size_hacspec  : int32 :=
+  @repr WORDSIZE32 1.
+(* Coq code:38 ends here *)
+
+(* [[file:concordium.org::*Coq code][Coq code:39]] *)
+Definition resize_state_hacspec (new_size_70 : int32) : int32 :=
+  @repr WORDSIZE32 1.
+(* Coq code:39 ends here *)
+
+(* [[file:concordium.org::*Coq code][Coq code:40]] *)
+Definition get_parameter_section_hacspec
+  (buf_71 : public_byte_seq)
+  (offset_72 : int32)
+  : (public_byte_seq × int32) :=
+  (buf_71, @repr WORDSIZE32 1).
+(* Coq code:40 ends here *)
+
+(* [[file:concordium.org::*Coq code][Coq code:41]] *)
+Definition get_parameter_size_hacspec  : int32 :=
+  @repr WORDSIZE32 1.
+(* Coq code:41 ends here *)
+
+(* [[file:concordium.org::*Coq code][Coq code:42]] *)
+Definition get_slot_time_hacspec  : int64 :=
+  @repr WORDSIZE64 1.
+(* Coq code:42 ends here *)
+
+(* [[file:concordium.org::*Coq code][Coq code:43]] *)
+Definition get_policy_section_hacspec
+  (policy_bytes_73 : public_byte_seq)
+  (offset_74 : int32)
+  : (public_byte_seq × int32) :=
+  (policy_bytes_73, @repr WORDSIZE32 1).
+(* Coq code:43 ends here *)
+
+(* [[file:concordium.org::*Coq code][Coq code:44]] *)
+Definition get_init_origin_hacspec
+  (start_75 : public_byte_seq)
+  : public_byte_seq :=
+  start_75.
+(* Coq code:44 ends here *)
+
+(* [[file:concordium.org::*Coq code][Coq code:45]] *)
+Definition get_receive_invoker_hacspec
+  (start_76 : public_byte_seq)
+  : public_byte_seq :=
+  start_76.
+(* Coq code:45 ends here *)
+
+(* [[file:concordium.org::*Coq code][Coq code:46]] *)
+Definition get_receive_self_address_hacspec
+  (start_77 : public_byte_seq)
+  : public_byte_seq :=
+  start_77.
+(* Coq code:46 ends here *)
+
+(* [[file:concordium.org::*Coq code][Coq code:47]] *)
+Definition get_receive_self_balance_hacspec  : int64 :=
+  @repr WORDSIZE64 1.
+(* Coq code:47 ends here *)
+
+(* [[file:concordium.org::*Coq code][Coq code:48]] *)
+Definition get_receive_sender_hacspec
+  (start_78 : public_byte_seq)
+  : public_byte_seq :=
+  start_78.
+(* Coq code:48 ends here *)
+
+(* [[file:concordium.org::*Coq code][Coq code:49]] *)
+Definition log_event_hacspec
+  (start_79 : public_byte_seq)
+  : (public_byte_seq × int32) :=
+  (start_79, @repr WORDSIZE32 1).
+(* Coq code:49 ends here *)
+
+(* [[file:concordium.org::*Coq code][Coq code:50]] *)
+Definition accept_hacspec  : int32 :=
+  @repr WORDSIZE32 1.
+(* Coq code:50 ends here *)
+
+(* [[file:concordium.org::*Coq code][Coq code:51]] *)
+Definition simple_transfer_hacspec
+  (buf_80 : public_byte_seq)
+  (amount_81 : int64)
+  : int32 :=
+  @repr WORDSIZE32 1.
+(* Coq code:51 ends here *)
+
+(* [[file:concordium.org::*Coq code][Coq code:52]] *)
+Definition send_hacspec
+  (addr_index_82 : int64)
+  (addr_subindex_83 : int64)
+  (receive_name_84 : public_byte_seq)
+  (amount_85 : int64)
+  (parameter_86 : public_byte_seq)
+  : int32 :=
+  @repr WORDSIZE32 1.
+(* Coq code:52 ends here *)
+
+(* [[file:concordium.org::*Coq code][Coq code:53]] *)
+Definition combine_and_hacspec (l_87 : int32) (r_88 : int32) : int32 :=
+  @repr WORDSIZE32 1.
+(* Coq code:53 ends here *)
+
+(* [[file:concordium.org::*Coq code][Coq code:54]] *)
+Definition combine_or_hacspec (l_89 : int32) (r_90 : int32) : int32 :=
+  @repr WORDSIZE32 1.
+(* Coq code:54 ends here *)
+
+(* [[file:concordium.org::*Coq code][Coq code:55]] *)
 Inductive log_error_t :=
 | Full : log_error_t
 | Malformed : log_error_t.
@@ -40,541 +562,5 @@ Proof. split. intros; destruct x ; destruct y ; try (f_equal ; apply eqb_leibniz
 Instance eq_dec_log_error_t : EqDec (log_error_t) :=
 Build_EqDec (log_error_t) (eqb_log_error_t) (eqb_leibniz_log_error_t).
 
-(* Coq code:5 ends here *)
-
-(* [[file:concordium.org::*Coq code][Coq code:6]] *)
-Require Import Hacspec.Lib.
-(* Coq code:6 ends here *)
-
-(* [[file:concordium.org::*Coq code][Coq code:7]] *)
-Definition load_state_hacspec
-  (buf_0 : public_byte_seq)
-  (offset_1 : int32)
-  : (public_byte_seq × int32) :=
-  (buf_0, @repr WORDSIZE32 1).
-(* Coq code:7 ends here *)
-
-(* [[file:concordium.org::*Coq code][Coq code:8]] *)
-Definition write_state_hacspec
-  (buf_2 : public_byte_seq)
-  (offset_3 : int32)
-  : (public_byte_seq × int32) :=
-  (buf_2, @repr WORDSIZE32 1).
-(* Coq code:8 ends here *)
-
-(* [[file:concordium.org::*Coq code][Coq code:9]] *)
-Definition state_size_hacspec  : int32 :=
-  @repr WORDSIZE32 1.
-(* Coq code:9 ends here *)
-
-(* [[file:concordium.org::*Coq code][Coq code:10]] *)
-Definition resize_state_hacspec (new_size_4 : int32) : int32 :=
-  @repr WORDSIZE32 1.
-(* Coq code:10 ends here *)
-
-(* [[file:concordium.org::*Coq code][Coq code:11]] *)
-Definition get_parameter_section_hacspec
-  (buf_5 : public_byte_seq)
-  (offset_6 : int32)
-  : (public_byte_seq × int32) :=
-  (buf_5, @repr WORDSIZE32 1).
-(* Coq code:11 ends here *)
-
-(* [[file:concordium.org::*Coq code][Coq code:12]] *)
-Definition get_parameter_size_hacspec  : int32 :=
-  @repr WORDSIZE32 1.
-(* Coq code:12 ends here *)
-
-(* [[file:concordium.org::*Coq code][Coq code:13]] *)
-Definition get_slot_time_hacspec  : int64 :=
-  @repr WORDSIZE64 1.
-(* Coq code:13 ends here *)
-
-(* [[file:concordium.org::*Coq code][Coq code:14]] *)
-Definition get_policy_section_hacspec
-  (policy_bytes_7 : public_byte_seq)
-  (offset_8 : int32)
-  : (public_byte_seq × int32) :=
-  (policy_bytes_7, @repr WORDSIZE32 1).
-(* Coq code:14 ends here *)
-
-(* [[file:concordium.org::*Coq code][Coq code:15]] *)
-Definition get_init_origin_hacspec
-  (start_9 : public_byte_seq)
-  : public_byte_seq :=
-  start_9.
-(* Coq code:15 ends here *)
-
-(* [[file:concordium.org::*Coq code][Coq code:16]] *)
-Definition get_receive_invoker_hacspec
-  (start_10 : public_byte_seq)
-  : public_byte_seq :=
-  start_10.
-(* Coq code:16 ends here *)
-
-(* [[file:concordium.org::*Coq code][Coq code:17]] *)
-Definition get_receive_self_address_hacspec
-  (start_11 : public_byte_seq)
-  : public_byte_seq :=
-  start_11.
-(* Coq code:17 ends here *)
-
-(* [[file:concordium.org::*Coq code][Coq code:18]] *)
-Definition get_receive_self_balance_hacspec  : int64 :=
-  @repr WORDSIZE64 1.
-(* Coq code:18 ends here *)
-
-(* [[file:concordium.org::*Coq code][Coq code:19]] *)
-Definition get_receive_sender_hacspec
-  (start_12 : public_byte_seq)
-  : public_byte_seq :=
-  start_12.
-(* Coq code:19 ends here *)
-
-(* [[file:concordium.org::*Coq code][Coq code:20]] *)
-Definition get_receive_owner_hacspec
-  (start_13 : public_byte_seq)
-  : public_byte_seq :=
-  start_13.
-(* Coq code:20 ends here *)
-
-(* [[file:concordium.org::*Coq code][Coq code:21]] *)
-Definition log_event_hacspec
-  (start_14 : public_byte_seq)
-  : (public_byte_seq × int32) :=
-  (start_14, @repr WORDSIZE32 1).
-(* Coq code:21 ends here *)
-
-(* [[file:concordium.org::*Coq code][Coq code:22]] *)
-Definition accept_hacspec  : int32 :=
-  @repr WORDSIZE32 1.
-(* Coq code:22 ends here *)
-
-(* [[file:concordium.org::*Coq code][Coq code:23]] *)
-Definition simple_transfer_hacspec
-  (buf_15 : public_byte_seq)
-  (amount_16 : int64)
-  : int32 :=
-  @repr WORDSIZE32 1.
-(* Coq code:23 ends here *)
-
-(* [[file:concordium.org::*Coq code][Coq code:24]] *)
-Definition send_hacspec
-  (addr_index_17 : int64)
-  (addr_subindex_18 : int64)
-  (receive_name_19 : public_byte_seq)
-  (amount_20 : int64)
-  (parameter_21 : public_byte_seq)
-  : int32 :=
-  @repr WORDSIZE32 1.
-(* Coq code:24 ends here *)
-
-(* [[file:concordium.org::*Coq code][Coq code:25]] *)
-Definition combine_and_hacspec (l_22 : int32) (r_23 : int32) : int32 :=
-  @repr WORDSIZE32 1.
-(* Coq code:25 ends here *)
-
-(* [[file:concordium.org::*Coq code][Coq code:26]] *)
-Definition combine_or_hacspec (l_24 : int32) (r_25 : int32) : int32 :=
-  @repr WORDSIZE32 1.
-(* Coq code:26 ends here *)
-
-(* [[file:concordium.org::*Coq code][Coq code:27]] *)
-Require Import Hacspec.Lib.
-(* Coq code:27 ends here *)
-
-(* [[file:concordium.org::*Coq code][Coq code:28]] *)
-Notation "'reject_hacspec_t'" := (int32) : hacspec_scope.
-(* Coq code:28 ends here *)
-
-(* [[file:concordium.org::*Coq code][Coq code:29]] *)
-Definition reject_impl_deafult  : reject_hacspec_t :=
-  min_v.
-(* Coq code:29 ends here *)
-
-(* [[file:concordium.org::*Coq code][Coq code:30]] *)
-Definition new_reject_impl (x_26 : int32) : (option int32) :=
-  (if ((x_26) <.? (@repr WORDSIZE32 0)):bool then (@Some int32 (x_26)) else (
-      @None int32)).
-(* Coq code:30 ends here *)
-
-(* [[file:concordium.org::*Coq code][Coq code:31]] *)
-Definition reject_impl_convert_from_unit  : reject_hacspec_t :=
-  (min_v) .+ (@repr WORDSIZE32 1).
-
-Theorem ensures_reject_impl_convert_from_unit : forall result_27 ,
-@reject_impl_convert_from_unit  = result_27 ->
-~ (result_27 = @repr WORDSIZE32 0).
-Proof. Admitted.
-(* Coq code:31 ends here *)
-
-(* [[file:concordium.org::*Coq code][Coq code:32]] *)
-Definition reject_impl_convert_from_parse_error  : reject_hacspec_t :=
-  (min_v) .+ (@repr WORDSIZE32 2).
-
-Theorem ensures_reject_impl_convert_from_parse_error : forall result_27 ,
-@reject_impl_convert_from_parse_error  = result_27 ->
-~ (result_27 = @repr WORDSIZE32 0).
-Proof. Admitted.
-(* Coq code:32 ends here *)
-
-(* [[file:concordium.org::*Coq code][Coq code:33]] *)
-Definition reject_impl_from_log_error
-  (le_28 : log_error_t)
-  : reject_hacspec_t :=
-  match le_28 with
-  | Full => (min_v) .+ (@repr WORDSIZE32 3)
-  | Malformed => (min_v) .+ (@repr WORDSIZE32 4)
-  end.
-
-Theorem ensures_reject_impl_from_log_error : forall result_27 (
-  le_28 : log_error_t),
-@reject_impl_from_log_error le_28 = result_27 ->
-~ (result_27 = @repr WORDSIZE32 0).
-Proof. Admitted.
-(* Coq code:33 ends here *)
-
-(* [[file:concordium.org::*Coq code][Coq code:34]] *)
-Inductive new_contract_name_error_t :=
-| NewContractNameErrorMissingInitPrefix : new_contract_name_error_t
-| NewContractNameErrorTooLong : new_contract_name_error_t
-| NewContractNameErrorContainsDot : new_contract_name_error_t
-| NewContractNameErrorInvalidCharacters : new_contract_name_error_t.
-(* Coq code:34 ends here *)
-
-(* [[file:concordium.org::*Coq code][Coq code:35]] *)
-Definition reject_impl_from_new_contract_name_error
-  (nre_29 : new_contract_name_error_t)
-  : reject_hacspec_t :=
-  match nre_29 with
-  | NewContractNameErrorMissingInitPrefix => (min_v) .+ (@repr WORDSIZE32 5)
-  | NewContractNameErrorTooLong => (min_v) .+ (@repr WORDSIZE32 6)
-  | NewContractNameErrorContainsDot => (min_v) .+ (@repr WORDSIZE32 9)
-  | NewContractNameErrorInvalidCharacters => (min_v) .+ (@repr WORDSIZE32 10)
-  end.
-
-Theorem ensures_reject_impl_from_new_contract_name_error : forall result_27 (
-  nre_29 : new_contract_name_error_t),
-@reject_impl_from_new_contract_name_error nre_29 = result_27 ->
-~ (result_27 = @repr WORDSIZE32 0).
-Proof. Admitted.
-(* Coq code:35 ends here *)
-
-(* [[file:concordium.org::*Coq code][Coq code:36]] *)
-Inductive new_receive_name_error_t :=
-| NewReceiveNameErrorMissingDotSeparator : new_receive_name_error_t
-| NewReceiveNameErrorTooLong : new_receive_name_error_t
-| NewReceiveNameErrorInvalidCharacters : new_receive_name_error_t.
-(* Coq code:36 ends here *)
-
-(* [[file:concordium.org::*Coq code][Coq code:37]] *)
-Definition reject_impl_from_new_receive_name_error
-  (nre_30 : new_receive_name_error_t)
-  : reject_hacspec_t :=
-  match nre_30 with
-  | NewReceiveNameErrorMissingDotSeparator => (min_v) .+ (@repr WORDSIZE32 7)
-  | NewReceiveNameErrorTooLong => (min_v) .+ (@repr WORDSIZE32 8)
-  | NewReceiveNameErrorInvalidCharacters => (min_v) .+ (@repr WORDSIZE32 11)
-  end.
-
-Theorem ensures_reject_impl_from_new_receive_name_error : forall result_27 (
-  nre_30 : new_receive_name_error_t),
-@reject_impl_from_new_receive_name_error nre_30 = result_27 ->
-~ (result_27 = @repr WORDSIZE32 0).
-Proof. Admitted.
-(* Coq code:37 ends here *)
-
-(* [[file:concordium.org::*Coq code][Coq code:38]] *)
-Notation "'contract_state_hacspec_t'" := (int32) : hacspec_scope.
-(* Coq code:38 ends here *)
-
-(* [[file:concordium.org::*Coq code][Coq code:39]] *)
-Inductive seek_from_hacspec_t :=
-| Start : int64 -> seek_from_hacspec_t
-| End : int64 -> seek_from_hacspec_t
-| Current : int64 -> seek_from_hacspec_t.
-(* Coq code:39 ends here *)
-
-(* [[file:concordium.org::*Coq code][Coq code:40]] *)
-Notation "'uint32_option_t'" := ((option int32)) : hacspec_scope.
-(* Coq code:40 ends here *)
-
-(* [[file:concordium.org::*Coq code][Coq code:41]] *)
-Notation "'iint64_option_t'" := ((option int64)) : hacspec_scope.
-(* Coq code:41 ends here *)
-
-(* [[file:concordium.org::*Coq code][Coq code:42]] *)
-Definition contract_state_impl_seek
-  (current_position_31 : contract_state_hacspec_t)
-  (pos_32 : seek_from_hacspec_t)
-  : (result (contract_state_hacspec_t × int64) unit) :=
-  match pos_32 with
-  | Start offset_33 => @Ok (contract_state_hacspec_t × int64) unit ((
-      @cast _ uint32 _ (offset_33),
-      offset_33
-    ))
-  | End delta_34 => (if ((delta_34) >=.? (@repr WORDSIZE64 0)):bool then (
-      match pub_uint32_checked_add (current_position_31) (@cast _ uint32 _ (
-          delta_34)) with
-      | Some b_35 => @Ok (contract_state_hacspec_t × int64) unit ((
-          b_35,
-          @cast _ uint64 _ (delta_34)
-        ))
-      | None => @Err (contract_state_hacspec_t × int64) unit (tt)
-      end) else (match pub_int64_checked_abs (delta_34) with
-      | Some b_36 => @Ok (contract_state_hacspec_t × int64) unit ((
-          (@repr WORDSIZE32 4) .- (@cast _ uint32 _ (b_36)),
-          @cast _ uint64 _ ((@repr WORDSIZE32 4) .- (@cast _ uint32 _ (b_36)))
-        ))
-      | None => @Err (contract_state_hacspec_t × int64) unit (tt)
-      end))
-  | Current delta_37 => (if ((delta_37) >=.? (@repr WORDSIZE64 0)):bool then (
-      match pub_uint32_checked_add (current_position_31) (@cast _ uint32 _ (
-          delta_37)) with
-      | Some offset_38 => @Ok (contract_state_hacspec_t × int64) unit ((
-          offset_38,
-          @cast _ uint64 _ (offset_38)
-        ))
-      | None => @Err (contract_state_hacspec_t × int64) unit (tt)
-      end) else (match pub_int64_checked_abs (delta_37) with
-      | Some b_39 => match pub_uint32_checked_sub (current_position_31) (
-        @cast _ uint32 _ (b_39)) with
-      | Some offset_40 => @Ok (contract_state_hacspec_t × int64) unit ((
-          offset_40,
-          @cast _ uint64 _ (offset_40)
-        ))
-      | None => @Err (contract_state_hacspec_t × int64) unit (tt)
-      end
-      | None => @Err (contract_state_hacspec_t × int64) unit (tt)
-      end))
-  end.
-(* Coq code:42 ends here *)
-
-(* [[file:concordium.org::*Coq code][Coq code:43]] *)
-Definition contract_state_impl_read_read
-  (current_position_41 : contract_state_hacspec_t)
-  (buf_42 : public_byte_seq)
-  : (contract_state_hacspec_t × uint_size) :=
-  let '(buf_43, num_read_44) :=
-    load_state_hacspec (buf_42) (current_position_41) in 
-  ((current_position_41) .+ (num_read_44), @cast _ uint32 _ (num_read_44)).
-(* Coq code:43 ends here *)
-
-(* [[file:concordium.org::*Coq code][Coq code:44]] *)
-Definition contract_state_impl_read_read_u64
-  (current_position_45 : contract_state_hacspec_t)
-  : (contract_state_hacspec_t × int64) :=
-  let buf_46 : seq int8 :=
-    seq_new_ (default) (usize 8) in 
-  let '(buf_47, num_read_48) :=
-    load_state_hacspec (buf_46) (current_position_45) in 
-  (
-    (current_position_45) .+ (num_read_48),
-    u64_from_le_bytes (array_from_seq (8) (buf_47))
-  ).
-(* Coq code:44 ends here *)
-
-(* [[file:concordium.org::*Coq code][Coq code:45]] *)
-Definition contract_state_impl_read_read_u32
-  (current_position_49 : contract_state_hacspec_t)
-  : (contract_state_hacspec_t × int32) :=
-  let buf_50 : seq int8 :=
-    seq_new_ (default) (usize 4) in 
-  let '(buf_51, num_read_52) :=
-    load_state_hacspec (buf_50) (current_position_49) in 
-  (
-    (current_position_49) .+ (num_read_52),
-    u32_from_le_bytes (array_from_seq (4) (buf_51))
-  ).
-(* Coq code:45 ends here *)
-
-(* [[file:concordium.org::*Coq code][Coq code:46]] *)
-Definition contract_state_impl_read_read_u8
-  (current_position_53 : contract_state_hacspec_t)
-  : (contract_state_hacspec_t × int8) :=
-  let buf_54 : seq int8 :=
-    seq_new_ (default) (usize 1) in 
-  let '(buf_55, num_read_56) :=
-    load_state_hacspec (buf_54) (current_position_53) in 
-  ((current_position_53) .+ (num_read_56), seq_index (buf_55) (usize 0)).
-(* Coq code:46 ends here *)
-
-(* [[file:concordium.org::*Coq code][Coq code:47]] *)
-Definition contract_state_impl_write
-  (current_position_57 : contract_state_hacspec_t)
-  (buf_58 : public_byte_seq)
-  : (result (contract_state_hacspec_t × uint_size) unit) :=
-  ifbnd option_is_none (pub_uint32_checked_add (current_position_57) (pub_u32 (
-        seq_len (buf_58)))) : bool
-  thenbnd (bind (@Err (contract_state_hacspec_t × uint_size) unit (tt)) (
-      fun _ =>  Ok (tt)))
-  else (tt) >> (fun 'tt =>
-  let '(buf_59, num_bytes_60) :=
-    write_state_hacspec (buf_58) (current_position_57) in 
-  @Ok (contract_state_hacspec_t × uint_size) unit ((
-      (current_position_57) .+ (num_bytes_60),
-      @cast _ uint32 _ (num_bytes_60)
-    ))).
-(* Coq code:47 ends here *)
-
-(* [[file:concordium.org::*Coq code][Coq code:48]] *)
-Definition has_contract_state_impl_for_contract_state_open
-  
-  : contract_state_hacspec_t :=
-  @repr WORDSIZE32 0.
-(* Coq code:48 ends here *)
-
-(* [[file:concordium.org::*Coq code][Coq code:49]] *)
-Definition has_contract_state_impl_for_contract_state_reserve
-  (contract_state_61 : contract_state_hacspec_t)
-  (len_62 : int32)
-  : bool :=
-  let cur_size_63 : int32 :=
-    state_size_hacspec  in 
-  (if ((cur_size_63) <.? (len_62)):bool then ((resize_state_hacspec (
-          len_62)) =.? (@repr WORDSIZE32 1)) else (true)).
-(* Coq code:49 ends here *)
-
-(* [[file:concordium.org::*Coq code][Coq code:50]] *)
-Definition has_contract_state_impl_for_contract_state_truncate
-  (current_position_64 : contract_state_hacspec_t)
-  (cur_size_65 : int32)
-  (new_size_66 : int32)
-  : contract_state_hacspec_t :=
-  let 'tt :=
-    if (cur_size_65) >.? (new_size_66):bool then (let _ : int32 :=
-        resize_state_hacspec (new_size_66) in 
-      tt) else (tt) in 
-  (if ((new_size_66) <.? (current_position_64)):bool then (new_size_66) else (
-      current_position_64)).
-(* Coq code:50 ends here *)
-
-(* [[file:concordium.org::*Coq code][Coq code:51]] *)
-Notation "'parameter_hacspec_t'" := (int32) : hacspec_scope.
-(* Coq code:51 ends here *)
-
-(* [[file:concordium.org::*Coq code][Coq code:52]] *)
-Definition read_impl_for_parameter_read
-  (current_position_67 : parameter_hacspec_t)
-  (buf_68 : public_byte_seq)
-  : (parameter_hacspec_t × uint_size) :=
-  let '(buf_69, num_read_70) :=
-    get_parameter_section_hacspec (buf_68) (current_position_67) in 
-  ((current_position_67) .+ (num_read_70), @cast _ uint32 _ (num_read_70)).
-(* Coq code:52 ends here *)
-
-(* [[file:concordium.org::*Coq code][Coq code:53]] *)
-Notation "'attributes_cursor_hacspec_t'" := ((int32 × int16)) : hacspec_scope.
-(* Coq code:53 ends here *)
-
-(* [[file:concordium.org::*Coq code][Coq code:54]] *)
-Definition has_policy_impl_for_policy_attributes_cursor_next_item
-  (policy_attribute_items_71 : attributes_cursor_hacspec_t)
-  (buf_72 : public_byte_seq)
-  : (option (attributes_cursor_hacspec_t × (int8 × int8))) :=
-  let '(current_position_73, remaining_items_74) :=
-    policy_attribute_items_71 in 
-  ifbnd (remaining_items_74) =.? (@repr WORDSIZE16 0) : bool
-  thenbnd (bind (@None (attributes_cursor_hacspec_t × (int8 × int8))) (
-      fun _ =>  Some (tt)))
-  else (tt) >> (fun 'tt =>
-  let '(tag_value_len_75, num_read_76) :=
-    get_policy_section_hacspec (seq_new_ (default) (usize 2)) (
-      current_position_73) in 
-  let current_position_73 :=
-    (current_position_73) .+ (num_read_76) in 
-  ifbnd (seq_index (tag_value_len_75) (usize 1)) >.? (@repr WORDSIZE8 31) : bool
-  thenbnd (bind (@None (attributes_cursor_hacspec_t × (int8 × int8))) (
-      fun _ =>  Some (tt)))
-  else (tt) >> (fun 'tt =>
-  let '(buf_77, num_read_78) :=
-    get_policy_section_hacspec (buf_72) (current_position_73) in 
-  let current_position_73 :=
-    (current_position_73) .+ (num_read_78) in 
-  let remaining_items_74 :=
-    (remaining_items_74) .- (@repr WORDSIZE16 1) in 
-  @Some (attributes_cursor_hacspec_t × (int8 × int8)) ((
-      (current_position_73, remaining_items_74),
-      (
-        seq_index (tag_value_len_75) (usize 0),
-        seq_index (tag_value_len_75) (usize 1)
-      )
-    )))).
-(* Coq code:54 ends here *)
-
-(* [[file:concordium.org::*Coq code][Coq code:55]] *)
-Notation "'policies_iterator_hacspec_t'" := ((int32 × int16)) : hacspec_scope.
 (* Coq code:55 ends here *)
-
-(* [[file:concordium.org::*Coq code][Coq code:56]] *)
-Notation "'policy_attributes_cursor_hacspec_t'" := ((
-  int32 ×
-  int64 ×
-  int64 ×
-  attributes_cursor_hacspec_t
-)) : hacspec_scope.
-(* Coq code:56 ends here *)
-
-(* [[file:concordium.org::*Coq code][Coq code:57]] *)
-Definition iterator_impl_for_policies_iterator_next
-  (policies_iterator_79 : policies_iterator_hacspec_t)
-  : (option (policies_iterator_hacspec_t × policy_attributes_cursor_hacspec_t
-    )) :=
-  let '(pos_80, remaining_items_81) :=
-    policies_iterator_79 in 
-  ifbnd (remaining_items_81) =.? (@repr WORDSIZE16 0) : bool
-  thenbnd (bind (@None (
-        policies_iterator_hacspec_t ×
-        policy_attributes_cursor_hacspec_t
-      )) (fun _ =>  Some (tt)))
-  else (tt) >> (fun 'tt =>
-  let '(buf_82, _) :=
-    get_policy_section_hacspec (seq_new_ (default) (((((usize 2) + (
-                usize 4)) + (usize 8)) + (usize 8)) + (usize 2))) (pos_80) in 
-  let skip_part_83 : public_byte_seq :=
-    seq_slice_range (buf_82) ((usize 0, usize 2)) in 
-  let ip_part_84 : public_byte_seq :=
-    seq_slice_range (buf_82) ((usize 2, (usize 2) + (usize 4))) in 
-  let created_at_part_85 : public_byte_seq :=
-    seq_slice_range (buf_82) ((
-        (usize 2) + (usize 4),
-        ((usize 2) + (usize 4)) + (usize 8)
-      )) in 
-  let valid_to_part_86 : public_byte_seq :=
-    seq_slice_range (buf_82) ((
-        ((usize 2) + (usize 4)) + (usize 8),
-        (((usize 2) + (usize 4)) + (usize 8)) + (usize 8)
-      )) in 
-  let len_part_87 : public_byte_seq :=
-    seq_slice_range (buf_82) ((
-        (((usize 2) + (usize 4)) + (usize 8)) + (usize 8),
-        ((((usize 2) + (usize 4)) + (usize 8)) + (usize 8)) + (usize 2)
-      )) in 
-  let identity_provider_88 : int32 :=
-    u32_from_le_bytes (array_from_seq (4) (ip_part_84)) in 
-  let created_at_89 : int64 :=
-    u64_from_le_bytes (array_from_seq (8) (created_at_part_85)) in 
-  let valid_to_90 : int64 :=
-    u64_from_le_bytes (array_from_seq (8) (valid_to_part_86)) in 
-  let remaining_items_91 : int16 :=
-    u16_from_le_bytes (array_from_seq (2) (len_part_87)) in 
-  let attributes_start_92 : int32 :=
-    (((((pos_80) .+ (@repr WORDSIZE32 2)) .+ (@repr WORDSIZE32 4)) .+ (
-          @repr WORDSIZE32 8)) .+ (@repr WORDSIZE32 8)) .+ (
-      @repr WORDSIZE32 2) in 
-  let pos_80 :=
-    ((pos_80) .+ (@cast _ uint32 _ (u16_from_le_bytes (array_from_seq (2) (
-              skip_part_83))))) .+ (@repr WORDSIZE32 2) in 
-  let remaining_items_91 :=
-    (remaining_items_91) .- (@repr WORDSIZE16 1) in 
-  @Some (policies_iterator_hacspec_t × policy_attributes_cursor_hacspec_t) ((
-      (pos_80, remaining_items_91),
-      (
-        identity_provider_88,
-        created_at_89,
-        valid_to_90,
-        (attributes_start_92, remaining_items_91)
-      )
-    ))).
-(* Coq code:57 ends here *)
 
